src/program_proof/marshal_proof.v
@@ -307,8 +307,8 @@ Proof.
   reflexivity.
 Qed.
 
-Theorem wp_Enc__PutInts stk E enc vs (s:Slice.t) (xs: list u64) :
-  {{{ is_enc enc vs ∗ is_slice_small s uint64T (u64val <$> xs) ∗
+Theorem wp_Enc__PutInts stk E enc vs (s:Slice.t) q (xs: list u64) :
+  {{{ is_enc enc vs ∗ is_slice_small s uint64T q (u64val <$> xs) ∗
              ⌜length (encode vs) + 8 * length xs <= int.val (EncSz enc)⌝ }}}
     Enc__PutInts (EncM.to_val enc) (slice_val s) @ stk; E
   {{{ RET #(); is_enc enc (vs ++ (EncUInt64 <$> xs)) }}}.
@@ -444,9 +444,9 @@ Proof.
   typeclasses eauto.
 Qed.
 
-Lemma array_to_block l (bs: list byte) :
+Lemma array_to_block l q (bs: list byte) :
   length bs = Z.to_nat 4096 ->
-  l ↦∗[byteT] (b2val <$> bs) -∗ mapsto_block l 1 (list_to_block bs).
+  l ↦∗[byteT]{q} (b2val <$> bs) -∗ mapsto_block l q (list_to_block bs).
 Proof.
   rewrite /array /mapsto_block /Block_to_vals /list_to_block.
   iIntros (H) "Hl".
@@ -466,7 +466,7 @@ Theorem wp_Enc__Finish stk E enc vs :
   {{{ is_enc enc vs }}}
     Enc__Finish (EncM.to_val enc) @ stk; E
   {{{ s (extra: list u8), RET (slice_val s);
-      is_slice_small s byteT (b2val <$> encode vs ++ extra) ∗
+      is_slice_small s byteT 1%Qp (b2val <$> encode vs ++ extra) ∗
       ⌜Slice.sz s = EncSz enc⌝ }}}.
 Proof.
   iIntros (Φ) "Henc HΦ".
@@ -502,7 +502,7 @@ Definition is_dec (dec: DecM.t) vs: iProp Σ :=
   ⌜(int.val off + length encoded + Z.of_nat (length extra))%Z = int.val (DecSz dec)⌝.
 
 Theorem wp_NewDec stk E s vs (extra: list u8) :
-  {{{ is_slice_small s byteT (b2val <$> encode vs ++ extra) }}}
+  {{{ is_slice_small s byteT 1%Qp (b2val <$> encode vs ++ extra) }}}
     NewDec (slice_val s) @ stk; E
   {{{ dec, RET (DecM.to_val dec); is_dec dec vs ∗ ⌜DecSz dec = s.(Slice.sz)⌝ }}}.
 Proof.
@@ -545,7 +545,7 @@ Proof.
   wp_store.
   wp_call.
   wp_apply wp_SliceSkip'; [ now len | ].
-  wp_apply (wp_UInt64Get' with "[Hx]").
+  wp_apply (wp_UInt64Get' _ _ _ 1%Qp with "[Hx]").
   { iSplitL.
     - cbn [Slice.ptr slice_skip].
       rewrite Z.mul_1_l.
@@ -603,7 +603,7 @@ Proof.
   wp_store.
   wp_call.
   wp_apply wp_SliceSkip'; [ now len | ].
-  wp_apply (wp_UInt32Get' with "[Hx]").
+  wp_apply (wp_UInt32Get' _ _ _ 1%Qp with "[Hx]").
   { iSplitL.
     - cbn [Slice.ptr slice_skip].
       rewrite Z.mul_1_l.
@@ -655,7 +655,7 @@ Qed.
 Theorem wp_Dec__GetInts stk E dec xs (n:u64) vs :
   {{{ is_dec dec ((EncUInt64 <$> xs) ++ vs) ∗ ⌜int.val n = length xs⌝}}}
     Dec__GetInts (DecM.to_val dec) #n @ stk; E
-  {{{ s, RET slice_val s; is_dec dec vs ∗ is_slice s uint64T (u64val <$> xs) }}}.
+  {{{ s, RET slice_val s; is_dec dec vs ∗ is_slice s uint64T 1%Qp (u64val <$> xs) }}}.
 Proof.
   rewrite /Dec__GetInts.
   iIntros (Φ) "(Hdec&%) HΦ".
@@ -673,7 +673,7 @@ Proof.
                         let remaining_xs: list u64 := drop num xs in
                         is_dec dec ((EncUInt64 <$> remaining_xs) ++ vs) ∗
                                ∃ s, l ↦[slice.T uint64T] (slice_val s) ∗
-                                    is_slice s uint64T (u64val <$> done_xs))%I with "[] [Hdec Hl Hli]").
+                                    is_slice s uint64T 1%Qp (u64val <$> done_xs))%I with "[] [Hdec Hl Hli]").
   - iIntros (i) "!>".
     clear Φ.
     iIntros (Φ) "([Hdec Hpre] & Hli & %) HΦ".
